icing/icing_optimisationsScript.sml
@@ -6,7 +6,7 @@
   icing_optimisationProofsScript.
 *)
 open bossLib;
-open fpValTreeTheory fpOptTheory;
+open fpOptTheory;
 
 open preamble;
 
@@ -20,7 +20,7 @@ End
   Generator for commutativity rewrites
 *)
 Definition fp_comm_gen_def:
-  fp_comm_gen op = (Binop op (Var 0) (Var 1), Binop op (Var 1) (Var 0))
+  fp_comm_gen op = (Binop op (PatVar 0) (PatVar 1), Binop op (PatVar 1) (PatVar 0))
 End
 
 (* Commutativity of + *)
@@ -35,8 +35,8 @@ val fp_mul_comm_def =
   Generator for associativity rewrites
 *)
 Definition fp_assoc_gen_def:
-  fp_assoc_gen op = (Binop op (Binop op (Var 0) (Var 1)) (Var 2),
-                     Binop op (Var 0) (Binop op (Var 1) (Var 2)))
+  fp_assoc_gen op = (Binop op (Binop op (PatVar 0) (PatVar 1)) (PatVar 2),
+                     Binop op (PatVar 0) (Binop op (PatVar 1) (PatVar 2)))
 End
 
 (* Associativity of + *)
@@ -67,14 +67,14 @@ val fp_mul_assoc2_def =
   FMA introudction
 *)
 Definition fp_fma_intro_def:
-  fp_fma_intro = (Binop FP_Add (Binop FP_Mul (Var 0) (Var 1)) (Var 2),
-                  Terop FP_Fma (Var 2) (Var 0) (Var 1))
+  fp_fma_intro = (Binop FP_Add (Binop FP_Mul (PatVar 0) (PatVar 1)) (PatVar 2),
+                  Terop FP_Fma (PatVar 2) (PatVar 0) (PatVar 1))
 End
 
 (* Subtraction -> Addition of inverse *)
 Definition fp_sub_add_def:
-  fp_sub_add = (Binop FP_Sub (Var 0) (Var 1),
-                Binop FP_Add (Var 0) (Unop FP_Neg (Var 1)))
+  fp_sub_add = (Binop FP_Sub (PatVar 0) (PatVar 1),
+                Binop FP_Add (PatVar 0) (Unop FP_Neg (PatVar 1)))
 End
 
 Definition fp_add_sub_def:
@@ -83,7 +83,7 @@ End
 
 Definition fp_times_minus_one_neg_def:
   (* 13830554455654793216 is -1.0 in binary representation *)
-  fp_times_minus_one_neg = (Binop FP_Mul (Var 0) (Word (13830554455654793216w: word64)), Unop FP_Neg (Var 0))
+  fp_times_minus_one_neg = (Binop FP_Mul (PatVar 0) (Word (13830554455654793216w: word64)), Unop FP_Neg (PatVar 0))
 End
 
 Definition fp_neg_times_minus_one_def:
@@ -94,51 +94,51 @@ End
 as the bottom-up traversal will not apply the rewrite otherwise *)
 Definition fp_neg_push_mul_r_def:
   fp_neg_push_mul_r =
-  (Binop FP_Add (Unop FP_Neg (Binop FP_Mul (Var 0) (Var 1))) (Var 2),
-   Binop FP_Add (Binop FP_Mul (Var 0) (Unop FP_Neg (Var 1))) (Var 2))
+  (Binop FP_Add (Unop FP_Neg (Binop FP_Mul (PatVar 0) (PatVar 1))) (PatVar 2),
+   Binop FP_Add (Binop FP_Mul (PatVar 0) (Unop FP_Neg (PatVar 1))) (PatVar 2))
 End
 
 Definition fp_times_two_to_add_def:
   (* 2.0 is 4611686018427387904 in binary representation *)
-  fp_times_two_to_add = (Binop FP_Mul (Var 0) (Word (4611686018427387904w: word64)),
-                         Binop FP_Add (Var 0) (Var 0))
+  fp_times_two_to_add = (Binop FP_Mul (PatVar 0) (Word (4611686018427387904w: word64)),
+                         Binop FP_Add (PatVar 0) (PatVar 0))
 End
 
 Definition fp_times_three_to_add_def:
   (* 3.0 is 4613937818241073152 in binary representation *)
-  fp_times_three_to_add = (Binop FP_Mul (Var 0) (Word (4613937818241073152w: word64)),
-                           Binop FP_Add (Binop FP_Add (Var 0) (Var 0)) (Var 0))
+  fp_times_three_to_add = (Binop FP_Mul (PatVar 0) (Word (4613937818241073152w: word64)),
+                           Binop FP_Add (Binop FP_Add (PatVar 0) (PatVar 0)) (PatVar 0))
 End
 
 Definition fp_times_zero_def:
-  fp_times_zero = (Binop FP_Mul (Var 0) (Word (0w: word64)), Word (0w: word64))
+  fp_times_zero = (Binop FP_Mul (PatVar 0) (Word (0w: word64)), Word (0w: word64))
 End
 
 Definition fp_plus_zero_def:
-  fp_plus_zero = (Binop FP_Add (Var 0) (Word (0w: word64)), (Var 0))
+  fp_plus_zero = (Binop FP_Add (PatVar 0) (Word (0w: word64)), (PatVar 0))
 End
 
 Definition fp_times_one_def:
   (* 4607182418800017408 is 1.0 in binary representation *)
-  fp_times_one = (Binop FP_Mul (Var 0) (Word (4607182418800017408w: word64)), (Var 0))
+  fp_times_one = (Binop FP_Mul (PatVar 0) (Word (4607182418800017408w: word64)), (PatVar 0))
 End
 
 Definition fp_times_into_div_def:
-  fp_times_into_div = (Binop FP_Mul (Binop FP_Div (Var 0) (Var 1)) (Var 2), Binop FP_Div (Binop FP_Mul (Var 0) (Var 2)) (Var 1))
+  fp_times_into_div = (Binop FP_Mul (Binop FP_Div (PatVar 0) (PatVar 1)) (PatVar 2), Binop FP_Div (Binop FP_Mul (PatVar 0) (PatVar 2)) (PatVar 1))
 End
 
 Definition fp_same_sub_def:
-  fp_same_sub = (Binop FP_Sub (Var 0) (Var 0), (Word (0w: word64)))
+  fp_same_sub = (Binop FP_Sub (PatVar 0) (PatVar 0), (Word (0w: word64)))
 End
 
 Definition fp_same_div_def:
   (* 4607182418800017408 is 1.0 in binary representation *)
-  fp_same_div = (Binop FP_Div (Var 0) (Var 0), (Word (4607182418800017408w: word64)))
+  fp_same_div = (Binop FP_Div (PatVar 0) (PatVar 0), (Word (4607182418800017408w: word64)))
 End
 
 Definition fp_distribute_gen_def:
-  fp_distribute_gen opInner opOuter = (Binop opOuter (Binop opInner (Var 0) (Var 2)) (Binop opInner (Var 1) (Var 2)),
-                                       Binop opInner (Binop opOuter (Var 0) (Var 1)) (Var 2))
+  fp_distribute_gen opInner opOuter = (Binop opOuter (Binop opInner (PatVar 0) (PatVar 2)) (Binop opInner (PatVar 1) (PatVar 2)),
+                                       Binop opInner (Binop opOuter (PatVar 0) (PatVar 1)) (PatVar 2))
 End
 
 (* Distributivity of * and + *)
