icing/icing_rewriterScript.sml
@@ -20,7 +20,7 @@ Definition matchesFPexp_def:
     | App FpFromWord [Lit (Word64 w2)] =>
       if (w1 = w2) then SOME s else NONE
     | _ => NONE) /\
-  (matchesFPexp (Var n) e s =
+  (matchesFPexp (PatVar n) e s =
     case substLookup s n of
     | SOME e1 => if e1 = e then SOME s else NONE
     | NONE => SOME (substAdd n e s)) /\
@@ -69,7 +69,7 @@ End
 (* Instantiate a given fp_pattern with a substitution into an expression *)
 Definition appFPexp_def:
   appFPexp (Word w) s = SOME (App FpFromWord [Lit (Word64 w)]) /\
-  appFPexp (Var n) s = substLookup s n /\
+  appFPexp (PatVar n) s = substLookup s n /\
   appFPexp (Unop u p) s = (do e <- appFPexp p s; return (App (FP_uop u) [e]); od) /\
   appFPexp (Binop op p1 p2) s =
     (case appFPexp p1 s of
@@ -100,7 +100,7 @@ End
 
 Definition isFpArithPat_def:
   isFpArithPat (Word w) = T ∧
-  isFpArithPat (Var n) = T ∧
+  isFpArithPat (PatVar n) = T ∧
   isFpArithPat (Unop u p) = isFpArithPat p ∧
   isFpArithPat (Binop b p1 p2) = (isFpArithPat p1 ∧ isFpArithPat p2) ∧
   isFpArithPat (Terop t p1 p2 p3) =
